%!TEX root = ../main.tex
\section{Deterministic base dynamics}
	\todo{translate this section}

\begin{equation} 
	\label{system_1} 
	\begin{aligned} 
		\dot{S_p} &= 
			-\beta_p S_p
			\frac{I_v}{N_v} + \tilde{r_1} L_p + \tilde{r_2} I_p  
		\\ 
		\dot{L_p} &= 
			\beta_p S_p
			\frac{I_v}{N_v} - b L_p - \tilde{r_1} L_p  
		\\ 
		\dot{I_p} &= 
			b L_p - \tilde{r_2} I_p  \\ 
		\dot{S_v} &= 
			-\beta_v S_v 
			\frac{I_p}{N_p} - \tilde{\gamma} S_v
			+(1-\theta) \mu  
		\\ 
		\dot{I_v} &= 
			\beta_v S_v \frac{I_p}{N_p} 
			- \tilde{\gamma} I_v
			+ \theta \mu 
	\end{aligned} 
\end{equation} 
\todo{Make a table for description of  all parameters}
\todo{Redact this conservation law to the entire system \eqref{system_1}.
Write a introductory paragraph to Thm 1}

\begin{theorem}\label{theorem_1}
	With the notation of ODE \eqref{system_1}, let
	\begin{equation*}
		\begin{aligned}
			N_v(t) &:= S_v(t) + I_v(t) 
		 	\\
		 	N_v^{\infty} &:= \frac{\mu}{\gamma}.
		 \end{aligned}
	\end{equation*}
	Then for any initial condition 
	$
		(S_p(0), L_p(0), I_p(0), S_v(0), I_v(0) )^\top
	 	\in {(0,\infty) \times (0, N^\infty_v)}
	$, she plant and vector total populations respectively satisfies
	\begin{equation*}
		\begin{aligned}
			& \frac{d N_p}{dt} =
				\frac{d}{dt}(S_p + L_p + I_p) = 0,
			\\
			& \lim_{t\to \infty}
				N_v(t) = N_v^{\infty}.
		\end{aligned}
	\end{equation*}
\end{theorem}

\todo{Why we want to normalize?}
We use the following variable change to normalize  \eqref{system_1}:
\begin{equation}
	\label{eqn:normalization}
	\begin{aligned}
		& x = \frac{S_p}{N_p},
		& y = \frac{L_p}{N_p},
		& z = \frac{I_p}{N_p},
		& v = \frac{I_p}{N_v},
		& w = \frac{I_v}{N_v} .
	\end{aligned}
\end{equation}

Then, deterministic system (\ref{system_1}) becomes
\begin{equation}
	\begin{aligned}
		\label{system_2}
		\dot{x} &=
			-\beta_p x w + \tilde{r_1} y + \tilde{r_2} z 
		\\
		\dot{y} &=
			\beta_p x w - (b + \tilde{r_1}) y 
		\\
		\dot{z} &=
			b y - \tilde{r_2} z 
		\\
		\dot{v} &=
			-\beta_v v z  +(1-\theta-v)\frac{\mu}{N_v} 
		\\
		\dot{w} &=
			\beta_v v z + (\theta-w) \frac{\mu}{N_v}
		\end{aligned}
\end{equation}


	Following ideas from [referencia], we quantify uncertinity in replanting rate of
plants, and  died rate of vector, $r_1$, $r_2$ and $\gamma$, to this end, we
perturb parameters  \todo{write here the parameters} $r_1 \dots$ whit a Winner
process to obtain a stochastic differential equation(SDE). Here, the 
perturbation describe stochastic environmental noise on each population. In
symbols $ dB(t)=B(t+dt)-B(t)$ denotes the increment of a standard Wiener
process, thus we perturb potentially replanting $r_1$, $r_2$, and vector death
$\gamma$ in the infinitiesimal time interval $[t, t + dt)$ by
\begin{equation}
	\label{eq1}
	\begin{aligned}
		{r}_1 dt \rightsquigarrow r_1 dt + \sigma_L dB(t),
		\\
		{r}_2 dt \rightsquigarrow r_2 dt + \sigma_Id B(t),
		\\
		\gamma dt \rightsquigarrow \gamma dt + \sigma_vd B(t).
	\end{aligned}
\end{equation}
\todo{Is the same Brownian motion for the three equations?}

	Note that right hand side of \eqref{eq1} is a random perturbations of parameters
$r_1$, $r_2$, $\gamma$, with mean
$
	\EX{r_1 dt + \sigma_L dB(t)}
$
and variance 
\todo{Note that here we will use the latex proba package, plase use the same
commands in the remain of the manuscript}
$
	\VarX{r_1 dt + \sigma_L dB(t)} = \sigma_L^2dt
$, 
$
	\mathbb{E}(\tilde{r}_2dt) = r_2dt
$ 
and
$
	Var(\tilde{r}_2dt) = \sigma_I^2dt
$ 
and 
$
	\mathbb{E}(\tilde{\gamma}dt) = \gamma dt
$ and 
$
	Var(\tilde{\gamma}dt) = \sigma_v^2dt
$.
%
Thus, we establish an stochastic extencion from deterministic tomato model 
\eqref{system_1} by the It\^{o} SDE

\begin{equation}
	\label{system_3}
	\begin{aligned}
		d S_p &=
			\left(
				-\beta_p S_p \frac{I_v}{N_v} + r_1 L_p + r_2 I_p
			\right)dt 
			+ (\sigma_L L_p
			+ 
			\sigma_I I_p)dB(t) 
		\\
		dL_p &=
			\left(
				\beta_p S_p \frac{I_v}{N_v} - b L_p - r_1 L_p
			\right) dt 
			- \sigma_L L_p dB(t) 
		\\
		d I_p &=
			\left(
				b L_p - r_2 I_p
			\right) dt 
			- \sigma_I I_p dB(t) 
		\\
		dS_v &=
			\left(
				-\beta_v S_v \frac{I_p}{N_p} - \gamma S_v  + (1-\theta) \mu
			\right)dt - \sigma_v S_v dB(t) 
		\\
		d I_v &=
			\left(
				\beta_v S_v \frac{I_p}{N_p} -\gamma I_v + \theta \mu
			\right) dt 
			- \sigma_v I_v dB(t).
	\end{aligned}
\end{equation}
Applyng the change of variable \eqref{eqn:normalization} to system (\ref{system_3}) results
\begin{equation}
	\begin{aligned}
	\label{system_4}
		d x(t) &=
			(-\beta_p x w + r_1 y + r_2 z) dt 
			+ (\sigma_L y + \sigma_I z) dB(t) 
		\\
		dy(t) &=
			(\beta_p x w - (b + r_1) y) dt 
			- \sigma_L y dB(t)
		\\
		dz(t) &=
			(b y - r_2 z) dt -\sigma_I z dB(t)
		\\
		dv(t) &=
			\left(
				-\beta_v v z + (1-\theta-v) 
				\frac{\mu}{N_v}
			\right) dt 
		\\
		dw(t) &=
			\left(
				\beta_v v z 
				+ (\theta-w) \frac{\mu}{N_v}
			\right) dt
	\end{aligned}
\end{equation}
